version native

gencertif/parser.ml
@@ -1,0 +1,248 @@
+open Str
+
+open Big_int
+
+let shift = 6
+
+let skip s n =
+     (String.sub s n (String.length s - n))
+
+let nhexa =regexp  "^N\\$="
+let shexa =regexp  "^S\\$="
+let rhexa =regexp  "^R\\$="
+let ahexa =regexp  "^A\\$="
+let bhexa =regexp  "^B\\$="
+let thexa =regexp  "^T\\$="
+let jhexa =regexp  "^J\\$="
+let t0hexa =regexp  "^Type=0"
+let t1hexa =regexp  "^Type=1"
+let t2hexa =regexp  "^Type=2"
+let t3hexa =regexp  "^Type=3"
+let t4hexa =regexp  "^Type=4"
+let hexa = regexp "-?[ABCDEF0123456789]*"
+
+let hexstring s =
+  let rec main rem s = 
+    if String.length s <= shift then
+     (add_big_int
+       (mult_big_int 
+         (power_int_positive_int 16 (String.length s))
+          rem)
+       (big_int_of_int (int_of_string ("0x" ^ s))))
+    else
+     main
+     (add_big_int
+       (mult_big_int 
+         (power_int_positive_int 16 shift)
+          rem)
+       (big_int_of_int (int_of_string ("0x" ^ (String.sub s 0 shift)))))
+     (skip s shift) in
+    let _ = string_match hexa s 0 in ();
+    let s1 = matched_string s in 
+    if (String.contains s1 '-') then
+      minus_big_int (main zero_big_int (skip s1 1))
+    else
+      main zero_big_int s1
+
+
+
+
+let rec comp2 r =
+   let (q, r) = quomod_big_int r (big_int_of_int 2) in
+     if eq_big_int r zero_big_int then
+       succ_big_int (comp2 q)
+     else zero_big_int
+
+let gsqr n1 r =
+  let f = div_big_int n1 r in
+  let (s1,r1) = quomod_big_int r
+               (mult_big_int (big_int_of_int 2) f) in
+  sqrt_big_int
+   (sub_big_int
+      (square_big_int r1)
+      (mult_big_int (big_int_of_int 8) s1))
+
+
+let n = ref zero_big_int
+let s = ref zero_big_int
+let r = ref zero_big_int
+let a = ref zero_big_int
+let b = ref zero_big_int
+let t = ref zero_big_int
+let j = ref zero_big_int
+let ty = ref (-1)
+let file = ref ""
+let co = ref stdout
+let sep = ref ""
+
+let pe s =
+  output_string !co s;
+  output_string !co "\n";
+  flush !co
+
+let change_sep () =
+  if !sep = "" then sep := "(" else
+  if !sep = "(" then sep := "::"
+
+let process_type() =
+  if !ty != -1 then
+    begin
+    if !ty = 4 then
+      let n  = !n in
+      let t  = !t in
+      let j  = !j in
+      let a  = 
+           mult_big_int 
+             (mult_big_int (big_int_of_int 3) j)
+             (sub_big_int (big_int_of_int 1728) j) in
+      let b = 
+           mult_big_int 
+             (mult_big_int (big_int_of_int 2) j)
+             (square_big_int (sub_big_int (big_int_of_int 1728) j)) in
+      let l = mod_big_int
+               (add_big_int (power_big_int_positive_int t 3)
+                  (add_big_int  (mult_big_int a t) b))
+                n in
+      let a = mod_big_int 
+                (mult_big_int a (square_big_int l)) n in
+      let b = mod_big_int 
+                (mult_big_int b (power_big_int_positive_int l 3)) n in
+      let x = mod_big_int (mult_big_int t l) n in
+      let y = mod_big_int (square_big_int l) n in
+      begin             
+       pe !sep;
+       pe ("(Ell_certif");
+       pe ((string_of_big_int n));
+       pe ((string_of_big_int !s));
+       pe ("((" ^ (string_of_big_int !r) ^ ",1)::nil)");
+       pe ((string_of_big_int a));
+       pe ((string_of_big_int b));
+       pe ((string_of_big_int x));
+       pe ((string_of_big_int y) ^ ")");
+       flush !co;
+       change_sep()
+      end
+    else if !ty = 3 then
+      let n  = !n in
+      let t  = !t in 
+      let a  = !a in
+      let b =  !b in
+      let l = mod_big_int
+               (add_big_int (power_big_int_positive_int t 3)
+                  (add_big_int  (mult_big_int a t) b))
+                n in
+      let a = mod_big_int 
+                (mult_big_int a (square_big_int l)) n in
+      let b = mod_big_int 
+                (mult_big_int b (power_big_int_positive_int l 3)) n in
+      let x = mod_big_int (mult_big_int t l) n in
+      let y = mod_big_int (square_big_int l) n in
+      
+      begin       
+       pe !sep;
+       pe ("(Ell_certif");
+       pe ((string_of_big_int n));
+       pe ((string_of_big_int !s));
+       pe ("((" ^ (string_of_big_int !r) ^ ",1)::nil)");
+       pe ((string_of_big_int a));
+       pe ((string_of_big_int b));
+       pe ((string_of_big_int x));
+       pe ((string_of_big_int y) ^ ")");
+       change_sep()
+      end
+    else if !ty = 1 then
+      begin   
+       pe !sep;         
+       pe ("(SPock_certif ");
+       pe ((string_of_big_int !n));
+       pe ((string_of_big_int !b));
+       pe ("((" ^ (string_of_big_int !r)  ^ ", 1)::nil))" );
+       flush !co;
+       change_sep()      
+      end
+    else if !ty = 0 then
+      begin             
+       pe (!sep ^ " (Proof_certif " ^ (string_of_big_int !n) ^
+            " prime" ^ (string_of_big_int !n)  ^ ") :: nil)).");
+       pe "exact_no_check (refl_equal true).";
+       pe "Time Qed.";
+       flush !co
+      end
+    else 
+      begin             
+       pe ("Type = " ^ (string_of_int !ty));
+       flush !co
+      end
+   end;
+   n := !r
+
+
+
+
+let rf f = 
+n :=  zero_big_int;
+s :=  zero_big_int;
+r :=  zero_big_int;
+a :=  zero_big_int;
+b :=  zero_big_int;
+t :=  zero_big_int;
+j :=  zero_big_int;
+ty:= (-1);
+file := "";
+co := stdout;
+sep := "";
+let ic = open_in f in
+  let line = ref "" in
+  try 
+    while true do
+    line := input_line ic; 
+
+    if string_match nhexa !line 0 then
+ (
+             n := hexstring (skip !line 3);
+           file := "prime" ^ (String.sub (string_of_big_int !n) 0 1) ^ ".v";
+             co := open_out !file;
+(*
+             pe "Require Import PocklingtonRefl.";
+             pe "Set Virtual Machine.";
+             pe "Open Local Scope positive_scope.";
+*)
+             pe ("Lemma prime" ^ (string_of_big_int !n) ^
+                ": prime  " ^ (string_of_big_int !n) ^ ".");
+             pe "apply (Pocklington_refl ";
+             r := !n)
+    else if string_match shexa !line 0 then 
+          s := (hexstring (skip !line 3))
+    else if string_match rhexa !line 0 then 
+          r := (hexstring (skip !line 3))
+    else if string_match ahexa !line 0 then 
+          a := (hexstring (skip !line 3))
+    else if string_match bhexa !line 0 then 
+          b := (hexstring (skip !line 3))
+    else if string_match thexa !line 0 then 
+          t := (hexstring (skip !line 3))
+    else if string_match jhexa !line 0 then 
+          j := (hexstring (skip !line 3))
+    else if string_match t0hexa !line 0 then 
+          (process_type();ty := 0;process_type())
+    else if string_match t1hexa !line 0 then 
+          (process_type(); ty := 1)
+    else if string_match t2hexa !line 0 then 
+          (process_type(); ty := 2;)
+    else if string_match t3hexa !line 0 then 
+          (process_type(); ty := 3)
+    else if string_match t4hexa !line 0 then 
+          (process_type();ty := 4)
+    done                 
+
+  with e ->              
+    close_in_noerr ic;   
+    close_out_noerr !co
+
+                         
+
+let _ = 
+  if (Array.length Sys.argv) == 2 then
+    rf Sys.argv.(1)
+  else print_string "o2v file.out";
+       print_newline()
